Add more examples

examples.v
@@ -1,3 +1,4 @@
+From iris.base_logic Require Export auth.
 From iris.program_logic Require Export weakestpre hoare.
 From iris.heap_lang Require Export lang.
 From iris.proofmode Require Import tactics.
@@ -6,31 +7,33 @@ From iris.heap_lang Require Import proofmode notation.
 Section examples.
  Context `{heapG Σ}.
 
- Definition local_state (f : expr) `{Closed [] f} : expr :=
-  (let: "l" := Alloc #0 in f;; !"l")%E.
+ Definition local_state : expr :=
+  (λ: "f", let: "l" := Alloc #0 in "f" #();; !"l")%E.
 
- Lemma wp_local_state f `{Closed [] f} : ∀ P Φ,
-  {{ heap_ctx ★ {{ P }} f {{ Φ }} ★ P }} local_state f {{v, v = #0 ★ ∃ w, Φ w}}.
+ Lemma wp_local_state (f : val) : ∀ P Φ,
+  {{ heap_ctx ★ {{ P }} f #() {{ Φ }} ★ P }}
+  local_state f {{v, v = #0 ★ ∃ w, Φ w}}.
  Proof.
   iIntros (P Φ) "!# (#Hctx & Hf & HP)". unfold local_state.
-  wp_alloc l as "Hl". wp_let. wp_bind f.
+  wp_value. wp_let.
+  wp_alloc l as "Hl". wp_let. wp_bind (f _).
   iApply wp_wand_l. iSplitL "Hl"; last by iApply "Hf".
   iIntros (w) "HΦ". wp_seq. wp_load; iSplit; first done. iExists _; done.
  Qed.
 
- Definition local_state_lifted (f : expr) `{Closed [] f} : expr :=
-  (let: "l" := Alloc #0 in λ: <>, f;; !"l")%E.
+ Definition local_state_lifted : expr :=
+  (λ: "f", let: "l" := Alloc #0 in λ: <>, "f" #();; !"l")%E.
 
- Lemma wp_local_state_lifted f `{Closed [] f} : ∀ P Φ,
-  heap_ctx ★ {{ P }} f {{ Φ }} ⊢
+ Lemma wp_local_state_lifted (f : val) : ∀ P Φ,
+  heap_ctx ★ {{ P }} f #() {{ Φ }} ⊢
   {{ True }} (local_state_lifted f)
    {{v, {{P}} (of_val v) #() {{u, u = #0 ★ ∃ w, Φ w}} }}.
  Proof.
   iIntros (P Φ) "[#Hctx #Hf]!# _". unfold local_state_lifted.
-  wp_alloc l as "Hl".
+  wp_lam. wp_alloc l as "Hl".
   iMod (inv_alloc (nroot .@ "local_state_lifted") _ (l ↦ #0)%I with "[Hl]")
    as "#Hinv"; first by iNext.
-  wp_let. iIntros "!# HP". wp_seq. wp_bind f.
+  wp_let. iIntros "!# HP". wp_seq. wp_bind (f _).
   iApply wp_wand_l. iSplitR; last by iApply "Hf".
   iIntros (w) "HΦ". wp_seq.
   iInv (nroot .@ "local_state_lifted") as "Hl" "Hcl".
@@ -38,4 +41,416 @@ Section examples.
   iModIntro. iSplit; first done. iExists _; done.
  Qed.
 
+ Definition shared_state : expr :=
+  (let: "l" := Alloc #0 in λ: "f", "f" #();; !"l")%E.
+
+ Lemma wp_shared_state :
+  heap_ctx ⊢
+  {{ True }} shared_state
+   {{v, ∀ (f : val) P Φ,
+        {{ {{ P }} f #() {{ Φ }} ★ P}} (of_val v) f {{u, u = #0 ★ ∃ w, Φ w}}
+   }}.
+ Proof.
+  iIntros "#Hctx !# _". unfold shared_state.
+  wp_alloc l as "Hl".
+  iMod (inv_alloc (nroot .@ "shared_state") _ (l ↦ #0)%I with "[Hl]")
+   as "#Hinv"; first by iNext.
+  wp_let.
+  iIntros (f P Φ) "!# [#Hf HP]". wp_let. wp_bind (f _).
+  iApply wp_wand_l. iSplitR; last by iApply "Hf".
+  iIntros (w) "HΦ". wp_seq.
+  iInv (nroot .@ "shared_state") as "Hl" "Hcl".
+  wp_load. iMod ("Hcl" with "[Hl]") as "_"; first by iNext.
+  iModIntro. iSplit; first done. iExists _; done.
+ Qed.
+
+ Lemma wp_shared_state_2 :
+  heap_ctx ⊢
+  {{ True }}
+   let: "g" := shared_state in "g" (λ: <>, "g" (λ: "x", "x");; #())
+  {{v, v = #0 }}.
+ Proof.
+  iIntros "#Hctx !# _".
+  wp_bind shared_state.
+  iApply wp_wand_l; iSplitL; last (iApply (wp_shared_state with "[]"); done).
+  iIntros (g) "#Hg". wp_let.
+  iAssert (□ (WP (λ: <>, g (λ: "x", "x") ;; #()) #() {{ v, v = #() }}))%I as "#Hg'".
+  - iIntros "!#". wp_lam.
+    iAssert (□ (WP (λ: "x", "x") #() {{ v, v = #() }}))%I as "#Hg''";
+     first by iIntros "!#"; wp_lam.
+    wp_bind (g _).
+    iApply wp_wand_r; iSplitL.
+    + iApply ("Hg" $! (λ: "x", "x")%V True%I with "[Hg'']").
+      iSplit; last done. iIntros "!# _"; done.
+    + iIntros (w) "[Hw _]"; by wp_seq.
+  - iApply wp_wand_r; iSplitL.
+    iApply ("Hg" $! (λ: <>, g (λ: "x", "x") ;; #())%V True%I with "[]").
+    iSplit; last done. iIntros "!# _"; done.
+    iIntros (w) "[Hw _]"; done.
+ Qed.
+
 End examples.
+
+Section Contradiction.
+
+ Definition shared_state_ZO : expr :=
+  (let: "l" := Alloc #0 in
+   λ: "f", "l" <- #0;; "f" #();; "l" <- #1;; "f" #();; !"l")%E.
+
+ Hypothesis wp_shared_state_ZO :
+  ∀ Σ {Hhp : heapG Σ},
+  heap_ctx ⊢
+  {{ True }} shared_state_ZO
+   {{v, ∀ (f : val) P Φ,
+        {{ {{ P }} f #() {{ Φ }} ★ P}} (of_val v) f {{u, u = #1 ★ ∃ w, Φ w}}
+   }}.
+
+ Lemma wp_shared_state_ZO_2 :
+  ∀ Σ {Hhp : heapG Σ},
+  heap_ctx ⊢
+  {{ True }}
+   let: "g" := shared_state_ZO in "g" (λ: <>, "g" (λ: "x", "x");; #())
+  {{v, v = #1 }}.
+ Proof.
+  iIntros (Σ Hhp) "#Hctx !# _".
+  specialize (wp_shared_state_ZO Σ Hhp).
+  wp_bind shared_state_ZO.
+  iApply wp_wand_l; iSplitL; last (iApply (wp_shared_state_ZO with "[]"); done).
+  iIntros (g) "#Hg". wp_let.
+  iAssert (□ (WP (λ: <>, g (λ: "x", "x") ;; #()) #() {{ v, v = #() }}))%I as "#Hg'".
+  - iIntros "!#". wp_lam.
+    iAssert (□ (WP (λ: "x", "x") #() {{ v, v = #() }}))%I as "#Hg''";
+     first by iIntros "!#"; wp_lam.
+    wp_bind (g _).
+    iApply wp_wand_r; iSplitL.
+    + iApply ("Hg" $! (λ: "x", "x")%V True%I with "[Hg'']").
+      iSplit; last done. iIntros "!# _"; done.
+    + iIntros (w) "[Hw _]"; by wp_seq.
+  - iApply wp_wand_r; iSplitL.
+    iApply ("Hg" $! (λ: <>, g (λ: "x", "x") ;; #())%V True%I with "[]").
+    iSplit; last done. iIntros "!# _"; done.
+    iIntros (w) "[Hw _]"; done.
+ Qed.
+
+ Lemma Fork_wp_shared_state_ZO_2 :
+  ∀ Σ {Hhp : heapG Σ},
+  heap_ctx ⊢
+  {{ True }}
+   let: "g" := shared_state_ZO in
+   Fork ("g" (λ: <>, "g" (λ: "x", "x");; #()));;
+     "g" (λ: <>, "g" (λ: "x", "x");; #())
+  {{v, v = #1 }}.
+ Proof.
+  iIntros (Σ Hhp) "#Hctx !# _".
+  specialize (wp_shared_state_ZO Σ Hhp).
+  wp_bind shared_state_ZO.
+  iApply wp_wand_l; iSplitL; last (iApply (wp_shared_state_ZO with "[]"); done).
+  iIntros (g) "#Hg". wp_let.
+  iAssert (□ (WP (λ: <>, g (λ: "x", "x") ;; #()) #() {{ v, v = #() }}))%I
+   as "#Hg'".
+  - iIntros "!#". wp_lam.
+    iAssert (□ (WP (λ: "x", "x") #() {{ v, v = #() }}))%I as "#Hg''";
+     first by iIntros "!#"; wp_lam.
+    wp_bind (g _).
+    iApply wp_wand_r; iSplitL.
+    + iApply ("Hg" $! (λ: "x", "x")%V True%I with "[Hg'']").
+      iSplit; last done. iIntros "!# _"; done.
+    + iIntros (w) "[Hw _]"; by wp_seq.
+  - wp_bind (Fork _).
+    iApply wp_wand_r; iSplitL.
+    + iApply (wp_fork _ _ (λ w, w = #())%I with "[]").
+      iNext; iSplit; first done.
+      iApply wp_wand_r; iSplitL.
+      iApply ("Hg" $! (λ: <>, g (λ: "x", "x") ;; #())%V True%I with "[]").
+      iSplit; last done. iIntros "!# _"; done.
+      iIntros (w) "[Hw _]"; done.
+    + iIntros (w) "Hw". wp_seq.
+      iApply wp_wand_r; iSplitL.
+      iApply ("Hg" $! (λ: <>, g (λ: "x", "x") ;; #())%V True%I with "[]").
+      iSplit; last done. iIntros "!# _"; done.
+      iIntros (w') "[Hw' _]"; done.
+ Qed.
+
+ From iris.heap_lang Require Import adequacy.
+ From iris.program_logic Require Import ectxi_language.
+ From iris.algebra Require Import gmap.
+
+ Let Σ : gFunctors := #[ heapΣ ].
+
+ Lemma Fork_wp_shared_state_ZO_2_adequate :
+   adequate (let: "g" := shared_state_ZO in
+   Fork ("g" (λ: <>, "g" (λ: "x", "x");; #()));;
+     "g" (λ: <>, "g" (λ: "x", "x");; #())) ∅ (λ w, w = #1).
+ Proof.
+  apply (@wp_adequacy Σ _ _). iIntros (?) "Hσ".
+  iMod (auth_alloc to_heap ownP heapN _ ∅ with "[Hσ]") as (γ) "[Hc Hs]"; auto.
+  - auto using to_heap_valid.
+  - iApply (@Fork_wp_shared_state_ZO_2 Σ (HeapG _ _ _ γ) with "[Hc] []");
+     last done.
+    rewrite /heap_ctx /auth_ctx; done.
+ Qed.
+
+ (* single thread step *)
+ Ltac SngTS :=
+  econstructor;
+    [match goal with
+     |- step ([?A], _) _ =>
+        eapply (step_atomic _ _ A _ _ _ [] [] []); simpl; eauto
+    end | ].
+ (* fist thread step *)
+ Ltac FTS :=
+  econstructor;
+    [match goal with
+     |- step ([?A; _], _) _ =>
+        eapply (step_atomic _ _ A _ _ _ [] [] [_]); simpl; eauto
+    end | ].
+
+ (* second thread step *)
+ Ltac STS :=
+  econstructor;
+    [match goal with
+     |- step ([_; ?A], _) _ =>
+        eapply (step_atomic _ _ A _ _ _ [] [_] []); simpl; eauto
+    end | ].
+
+ Ltac to_val_handle_closed :=
+  simpl;
+    match goal with
+     |- match decide ?A with _ => _ end = _ =>
+        assert A by apply _; let c := fresh in
+         destruct (decide A) as [c|]; last tauto;
+         match type of c with
+          Closed ?A ?B => let e := W.of_expr B in
+           replace c with (W.is_closed_correct A e I);
+           first done; apply closed_proof_irrel
+         end
+       end.
+
+ Theorem InConsistent_wp_shared_state_ZO : False.
+ Proof.
+  pose proof (Fork_wp_shared_state_ZO_2_adequate) as [Ha _]. simpl in *.
+  cut (∃ e, rtc step
+         ([(let: "g" := shared_state_ZO
+            in Fork ("g" (λ: <>, "g" (λ: "x", "x") ;; #())) ;;
+            "g" (λ: <>, "g" (λ: "x", "x") ;; #()))%E], ∅)
+         ((of_val #0) :: [e], {[1%positive := #0]})).
+  + intros [e Hstp]. specialize (Ha _ _ _ Hstp). done.
+  + unfold shared_state_ZO.
+    eexists.
+    SngTS.
+    eapply (Ectx_step _ _ _ _ [] [AppRCtx (λ: "g", _); AppRCtx (λ: "l", _)]
+      (ref #0)%E (Lit $ LitLoc 1%positive)); eauto.
+    eapply AllocS; first done. by rewrite lookup_empty. simpl.
+    SngTS.
+    eapply (Ectx_step _ _ _ _ [] [AppRCtx (λ: "g", _)]
+      (_ (Lit $ LitLoc 1%positive))%E _); eauto; simpl.
+    eapply BetaS; eauto. typeclasses eauto. rewrite /= /subst /=.
+    SngTS.
+    eapply (Ectx_step _ _ _ _ [] [] _ _); eauto; simpl.
+    eapply BetaS; eauto; last typeclasses eauto.
+    to_val_handle_closed.
+    rewrite /= /subst /=.
+    econstructor;
+    [match goal with
+     |- step ([?A], _) _ =>
+        eapply (step_atomic _ _ A _ _ _ [_] [] []); simpl; eauto
+    end | ].
+    eapply (Ectx_step _ _ _ _ [_] [AppRCtx (λ: <>, _)] _ _); eauto; simpl.
+    eapply ForkS. simpl.
+    FTS.
+    eapply (Ectx_step _ _ _ _ [] [] _ _); eauto; simpl.
+    eapply BetaS; eauto; last typeclasses eauto.
+    simpl.
+    FTS.
+    eapply (Ectx_step _ _ _ _ [] [] _ _); eauto; simpl.
+    eapply BetaS; eauto; last typeclasses eauto.
+    to_val_handle_closed.
+    rewrite /= /subst /=.
+    FTS.
+    eapply (Ectx_step _ _ _ _ [] [AppRCtx (λ: <>, _)] _ _); eauto; simpl.
+    eapply StoreS; first done.
+    rewrite lookup_insert; eauto.
+    simpl.
+    FTS.
+    eapply (Ectx_step _ _ _ _ [] [] _ _); eauto; simpl.
+    eapply BetaS; eauto; last typeclasses eauto.
+    rewrite /= /subst /=.
+    FTS.
+    eapply (Ectx_step _ _ _ _ [] [AppRCtx (λ: <>, _)] _ _); eauto; simpl.
+    eapply BetaS; eauto; last typeclasses eauto.
+    rewrite /= /subst /=.
+    FTS.
+    eapply (Ectx_step _ _ _ _ [] [AppRCtx (λ: <>, _); AppRCtx (λ: <>, _)] _ _);
+     eauto; simpl.
+    eapply BetaS; eauto; last typeclasses eauto.
+    to_val_handle_closed.
+    rewrite /= /subst /=.
+    FTS.
+    eapply (Ectx_step _ _ _ _ []
+     [AppRCtx (λ: <>, _); AppRCtx (λ: <>, _); AppRCtx (λ: <>, _)] _ _);
+     eauto; simpl.
+    eapply StoreS; first done.
+    rewrite lookup_insert; eauto.
+    simpl.
+    FTS.
+    eapply (Ectx_step _ _ _ _ []
+     [AppRCtx (λ: <>, _); AppRCtx (λ: <>, _)] _ _);
+     eauto; simpl.
+    eapply BetaS; eauto; last typeclasses eauto.
+    rewrite /= /subst /=.
+    FTS.
+    eapply (Ectx_step _ _ _ _ []
+      [AppRCtx (λ: <>, _); AppRCtx (λ: <>, _); AppRCtx (λ: <>, _)] _ _);
+     eauto; simpl.
+    eapply BetaS; eauto; last typeclasses eauto.
+    rewrite /= /subst /=.
+    FTS.
+    eapply (Ectx_step _ _ _ _ []
+     [AppRCtx (λ: <>, _); AppRCtx (λ: <>, _)] _ _);
+     eauto; simpl.
+    eapply BetaS; eauto; last typeclasses eauto.
+    rewrite /= /subst /=.
+    FTS.
+    eapply (Ectx_step _ _ _ _ []
+      [AppRCtx (λ: <>, _); AppRCtx (λ: <>, _); AppRCtx (λ: <>, _)] _ _);
+     eauto; simpl.
+    eapply StoreS; first done.
+    rewrite lookup_insert; eauto.
+    simpl.
+    FTS.
+    eapply (Ectx_step _ _ _ _ []
+     [AppRCtx (λ: <>, _); AppRCtx (λ: <>, _)] _ _);
+     eauto; simpl.
+    eapply BetaS; eauto; last typeclasses eauto.
+    rewrite /= /subst /=.
+    FTS.
+    eapply (Ectx_step _ _ _ _ []
+     [AppRCtx (λ: <>, _); AppRCtx (λ: <>, _); AppRCtx (λ: <>, _)] _ _);
+     eauto; simpl.
+    eapply BetaS; eauto; last typeclasses eauto.
+    rewrite /= /subst /=.
+    FTS.
+    eapply (Ectx_step _ _ _ _ []
+     [AppRCtx (λ: <>, _); AppRCtx (λ: <>, _)] _ _);
+     eauto; simpl.
+    eapply BetaS; eauto; last typeclasses eauto.
+    rewrite /= /subst /=.
+    FTS.
+    eapply (Ectx_step _ _ _ _ []
+     [AppRCtx (λ: <>, _); AppRCtx (λ: <>, _)] _ _);
+     eauto; simpl.
+    eapply LoadS; eauto.
+    rewrite /= /subst /=.
+    FTS.
+    eapply (Ectx_step _ _ _ _ [] [AppRCtx (λ: <>, _)] _ _); eauto; simpl.
+    eapply BetaS; eauto; last typeclasses eauto.
+    rewrite /= /subst /=.
+    FTS.
+    eapply (Ectx_step _ _ _ _ [] [] _ _); eauto; simpl.
+    eapply BetaS; eauto; last typeclasses eauto.
+    rewrite /= /subst /=.
+    FTS.
+    eapply (Ectx_step _ _ _ _ [] [AppRCtx (λ: <>, _)] _ _); eauto; simpl.
+    eapply StoreS; first done.
+    rewrite lookup_insert; eauto.
+    simpl.
+    FTS.
+    eapply (Ectx_step _ _ _ _ [] [] _ _); eauto; simpl.
+    eapply BetaS; eauto; last typeclasses eauto.
+    rewrite /= /subst /=.
+    FTS.
+    eapply (Ectx_step _ _ _ _ [] [AppRCtx (λ: <>, _)] _ _); eauto; simpl.
+    eapply BetaS; eauto; last typeclasses eauto.
+    rewrite /= /subst /=.
+    FTS.
+    eapply (Ectx_step _ _ _ _ []
+     [AppRCtx (λ: <>, _); AppRCtx (λ: <>, _)] _ _); eauto; simpl.
+    eapply BetaS; eauto; last typeclasses eauto.
+    to_val_handle_closed.
+    rewrite /= /subst /=.
+    FTS.
+    eapply (Ectx_step _ _ _ _ []
+      [AppRCtx (λ: <>, _); AppRCtx (λ: <>, _); AppRCtx (λ: <>, _)] _ _);
+     eauto; simpl.
+    eapply StoreS; first done.
+    rewrite lookup_insert; eauto.
+    simpl.
+    FTS.
+    eapply (Ectx_step _ _ _ _ []
+     [AppRCtx (λ: <>, _); AppRCtx (λ: <>, _)] _ _);
+     eauto; simpl.
+    eapply BetaS; eauto; last typeclasses eauto.
+    rewrite /= /subst /=.
+    FTS.
+    eapply (Ectx_step _ _ _ _ []
+     [AppRCtx (λ: <>, _); AppRCtx (λ: <>, _); AppRCtx (λ: <>, _)] _ _);
+     eauto; simpl.
+    eapply BetaS; eauto; last typeclasses eauto.
+    rewrite /= /subst /=.
+    FTS.
+    eapply (Ectx_step _ _ _ _ []
+     [AppRCtx (λ: <>, _); AppRCtx (λ: <>, _)] _ _);
+     eauto; simpl.
+    eapply BetaS; eauto; last typeclasses eauto.
+    rewrite /= /subst /=.
+    FTS.
+    eapply (Ectx_step _ _ _ _ []
+     [AppRCtx (λ: <>, _); AppRCtx (λ: <>, _); AppRCtx (λ: <>, _)] _ _);
+     eauto; simpl.
+    eapply StoreS; first done.
+    rewrite lookup_insert; eauto.
+    rewrite /= /subst /=.
+    FTS.
+    eapply (Ectx_step _ _ _ _ []
+     [AppRCtx (λ: <>, _); AppRCtx (λ: <>, _)] _ _); eauto; simpl.
+    eapply BetaS; eauto; last typeclasses eauto.
+    rewrite /= /subst /=.
+    FTS.
+    eapply (Ectx_step _ _ _ _ []
+     [AppRCtx (λ: <>, _); AppRCtx (λ: <>, _); AppRCtx (λ: <>, _)] _ _);
+     eauto; simpl.
+    eapply BetaS; eauto; last typeclasses eauto.
+    rewrite /= /subst /=.
+    FTS.
+    eapply (Ectx_step _ _ _ _ []
+     [AppRCtx (λ: <>, _); AppRCtx (λ: <>, _)] _ _); eauto; simpl.
+    eapply BetaS; eauto; last typeclasses eauto.
+    rewrite /= /subst /=.
+    FTS.
+    eapply (Ectx_step _ _ _ _ []
+     [AppRCtx (λ: <>, _); AppRCtx (λ: <>, _)] _ _); eauto; simpl.
+    eapply LoadS; eauto.
+    rewrite /= /subst /=.
+    FTS.
+    eapply (Ectx_step _ _ _ _ [] [AppRCtx (λ: <>, _)] _ _); eauto; simpl.
+    eapply BetaS; eauto; last typeclasses eauto.
+    rewrite /= /subst /=.
+    FTS.
+    eapply (Ectx_step _ _ _ _ [] [] _ _); eauto; simpl.
+    eapply BetaS; eauto; last typeclasses eauto.
+    rewrite /= /subst /=.
+    STS.
+    eapply (Ectx_step _ _ _ _ [] [] _ _); eauto; simpl.
+    eapply BetaS; eauto; last typeclasses eauto.
+    to_val_handle_closed.
+    rewrite /= /subst /=.
+    STS.
+    eapply (Ectx_step _ _ _ _ [] [AppRCtx (λ: <>, _)] _ _); eauto; simpl.
+    eapply StoreS; first done.
+    rewrite lookup_insert; eauto.
+    rewrite /= /subst /=.
+    FTS.
+    eapply (Ectx_step _ _ _ _ [] [] _ _); eauto; simpl.
+    eapply LoadS; eauto.
+    rewrite /= /subst /=.
+    (* done *)
+    match goal with
+     |- rtc step ([_; _], ?A) ([_; _], ?B) => replace A with B
+    end.
+    apply rtc_refl.
+    apply map_eq => i. destruct (decide (i = 1%positive)); subst.
+    - by rewrite !lookup_insert.
+    - by rewrite !lookup_insert_ne.
+ Qed.
+
+End Contradiction.
